seq refactoring

Pom/Lpo/Operations/Seq.lean
@@ -1,183 +1,9 @@
-import Pcol.Semantics.Lpo.Basic
-import Pcol.Semantics.Lpo.FinApprox
-import Pcol.Semantics.Lpo.Order
+import Pom.Lpo.Operations.Seq.Branches
+import Pom.Lpo.Operations.Seq.Equiv
 
 namespace Lpofin
-open Classical
 
 variable {l : Type} [PartialOrder l] [OrderBot l]
-
--- stuck is a path condition formula indicating that the execution will definitely
--- encounter a ⊥ node
-def stuck (α : Lpofin l) : Form Node := Form.sOr fun x : ↑α.val.bots ↦ α.form x.val
-
-lemma stuck_antitone : @Antitone (Lpofin l) _ _ _ stuck := by
-  intro α β hle v ⟨⟨x, hx, hlab⟩, hform⟩
-  rcases hle.succ _ hx with hx' | ⟨y, ⟨hy, hlab'⟩, hyx⟩
-  · refine ⟨⟨x, hx', ?_⟩, ?_⟩
-    · refine le_antisymm ?_ bot_le
-      rw [← hlab]; exact hle.lab x
-    · refine (congrFun (hle.form x hx') v).mpr ?_
-      exact hform
-  · refine ⟨⟨y, hy, hlab'⟩, ?_⟩
-    refine (congrFun (hle.form _ hy) _).mpr ?_
-    refine (β.val.property.form _ (hle.nodes hy)).2 _ hyx _ ?_
-    exact hform
-
--- A node is in the exntensible set if it is possible for it not be stuck
-noncomputable def extens (α : Lpofin l) : Finset Node :=
-  α.nodes_finset.filter fun x ↦ ¬ α.form x ≤ α.stuck
-
-lemma extens_not_bot {α : Lpofin l} {x : Node} : x ∈ α.extens → α.lab x ≠ ⊥ := by
-  intro h; simp [extens] at h; intro heq; apply h.2; intro v hform
-  refine ⟨⟨x, ?_, heq⟩, hform⟩
-  exact (α.val.property.form_dom x).mp ⟨v, hform⟩
-
-lemma extens_subset_nodes {α : Lpofin l} : ∀ x ∈ α.extens, x ∈ α.nodes := by
-  intro x hx; exact (Set.Finite.mem_toFinset _).mp (Finset.mem_filter.mp hx).1
-
-lemma extens_monotone : @Monotone (Lpofin l) _ _ _ extens := by
-  intro α β hle x; simp [extens]; intro hx hstuck
-  have hx' := (Set.Finite.mem_toFinset _).mp hx
-  refine ⟨(Set.Finite.mem_toFinset _).mpr (hle.nodes hx'), fun hc ↦ ?_⟩
-  refine hstuck (fun v hform ↦ stuck_antitone hle v (hc v ?_))
-  simp [Lpofin.form]; rw [← hle.form x hx']; exact hform
-
-lemma le_extens {α β : Lpofin l} (hle : α ≤ β) :
-    α.extens = β.extens.filter fun x ↦ ¬ (β.form x ≤ α.stuck) := by
-  ext x; constructor
-  · intro hx; refine Finset.mem_filter.mpr ⟨extens_monotone hle hx, ?_⟩
-    intro c; refine (Finset.mem_filter.mp hx).2 (le_trans ?_ c)
-    exact le_form hle
-  · intro hx; obtain ⟨hx, hstk⟩ := Finset.mem_filter.mp hx
-    obtain ⟨hx', _⟩ := Finset.mem_filter.mp hx
-    apply (Set.Finite.mem_toFinset _).mp at hx'
-    rcases hle.succ _  hx' with hxα | ⟨y, ⟨hy, hbot⟩, hyx⟩
-    · refine Finset.mem_filter.mpr ⟨(Set.Finite.mem_toFinset _).mpr hxα, ?_⟩
-      intro c; refine hstk (le_of_eq_of_le (Eq.symm ?_) c)
-      exact hle.form _ hxα
-    · exfalso; refine hstk (((β.val.property.form y (hle.nodes hy)).2 _ hyx).trans ?_)
-      refine le_of_eq_of_le (Eq.symm (hle.form _ hy)) ?_
-      intro v hform; exact ⟨⟨y, hy, hbot⟩, hform⟩
-
-def conj (α : Lpofin l) (S : Finset Node) : Form Node :=
-  Form.sAnd fun x : ↑S ↦ α.form x.val
-
-def branches_set (α : Lpofin l) : Set (Form Node) :=
-  α.conj ''
-  { S : Finset Node
-  | S.Nonempty ∧
-    S ⊆ α.extens ∧
-    (α.conj S).sat ∧
-    α.conj S ≤ α.stuck.not ∧
-    ∀ T, S ⊂ T → T ⊆ α.extens → ¬ Form.sat (fun v ↦ ∀ x ∈ T, α.form x v)
-  }
-
-lemma branches_finite (α : Lpofin l) : α.branches_set.Finite := by
-  refine Set.Finite.image _ ?_
-  refine Set.Finite.subset α.extens.powerset.finite_toSet ?_
-  intro s ⟨_, hsub, _⟩; simp only [Finset.coe_powerset, Set.mem_preimage, Set.mem_powerset_iff,
-    Finset.coe_subset, hsub]
-
-noncomputable def branches (α : Lpofin l) : Finset (Form Node) := α.branches_finite.toFinset
-
-lemma branches_set_monotone : @Monotone (Lpofin l) _ _ _ branches_set := by
-  rintro α β hle φ ⟨S, ⟨hne, hsub, hsat, hstuck, hmax⟩, hφ⟩; subst hφ
-  refine ⟨S, ⟨hne, ?_, ?_, ?_, ?_⟩, ?_⟩
-  · exact le_trans hsub (extens_monotone hle)
-  · rcases hsat with ⟨v, hv⟩; use v; intro x
-    refine (congrFun (hle.form x ?_) _).mp (hv x)
-    have hx' := Finset.mem_of_mem_filter _ (hsub x.property)
-    exact (Set.Finite.mem_toFinset _).mp hx'
-  · intro v hform hstuck'; refine hstuck v ?_ ?_
-    · intro x; refine (congr_fun (hle.form x ?_) v).mpr (hform x)
-      have hx' := Finset.mem_of_mem_filter _ (hsub x.property)
-      exact (Set.Finite.mem_toFinset _).mp hx'
-    · exact stuck_antitone hle v hstuck'
-  · intro T hST hT ⟨v, hc⟩; obtain ⟨x, hxT, hxS⟩ := Finset.exists_of_ssubset hST
-    have hform : α.conj S v := by
-      intro y; refine (congrFun (hle.form _ ?_) _).mpr (hc _ ?_)
-      · exact extens_subset_nodes _ (hsub y.property)
-      · exact (Finset.ssubset_def.mp hST).1 y.property
-    rcases hle.succ _ (extens_subset_nodes _ (hT hxT))
-      with hx | ⟨y, hy, hyx⟩
-    · refine hmax (insert x S) (Finset.ssubset_insert hxS) ?_ ?_
-      · refine Finset.insert_subset (Finset.mem_filter.mpr ⟨?_, ?_⟩) hsub
-        · exact (Set.Finite.mem_toFinset _).mpr hx
-        · intro c; refine hstuck v hform ?_
-          exact c v ((congrFun (hle.form _ hx) _).mpr (hc _ hxT))
-      · use v; intro y hy; rcases Finset.mem_insert.mp hy with rfl | hy'
-        · exact (congrFun (hle.form y hx) _).mpr (hc y hxT)
-        · refine (congrFun (hle.form y ?_) _).mpr (hc y ?_)
-          · exact extens_subset_nodes _ (hsub hy')
-          · exact Finset.mem_of_subset (Finset.ssubset_def.mp hST).1 hy'
-    · refine hstuck v hform ⟨⟨y, hy⟩, ?_⟩
-      refine (congrFun (hle.form _ hy.1) _).mpr ?_
-      exact (β.val.property.form _ (hle.nodes hy.1)).2 _ hyx v (hc _ hxT)
-  · ext1 v; refine forall_congr fun x ↦ ?_; ext; constructor
-    · intro h; refine (congr_fun (hle.form x ?_) v).mpr h
-      have hx' := Finset.mem_of_mem_filter _ (hsub x.property)
-      exact (Set.Finite.mem_toFinset _).mp hx'
-    · intro h; refine (congr_fun (hle.form x ?_) v).mp h
-      have hx' := Finset.mem_of_mem_filter _ (hsub x.property)
-      exact (Set.Finite.mem_toFinset _).mp hx'
-
-lemma le_branches_set {α β : Lpofin l} (hle : α ≤ β) :
-    α.branches_set = { φ ∈ β.branches_set | φ ≤ α.stuck.not } := by
-  ext φ; constructor
-  · intro h; constructor
-    · exact branches_set_monotone hle h
-    · rcases h with ⟨_, ⟨_, _, _, hstuck, _⟩, rfl⟩
-      exact hstuck
-  · rintro ⟨⟨S, ⟨hne, hsub, ⟨v, hsat⟩, _, hmax⟩, rfl⟩, hstuck⟩
-    have hS x (hx : x ∈ S) : x ∈ α.nodes := by
-      have hx' := extens_subset_nodes _ (hsub hx)
-      rcases hle.succ _ hx' with hxα | ⟨y, hbot, hyx⟩
-      · exact hxα
-      · exfalso; refine forall_not_of_not_exists (hstuck v hsat) ⟨y, hbot⟩ ?_
-        refine (congrFun (hle.form y hbot.1) _).mpr ?_
-        refine (β.val.property.form y (hle.nodes hbot.1)).2 _ hyx v ?_
-        exact hsat ⟨_, hx⟩
-    refine ⟨S, ⟨hne, ?_, ⟨v, ?_⟩, ?_, ?_⟩, ?_⟩
-    · intro x hx; rw [le_extens hle]; refine Finset.mem_filter.mpr ⟨?_, ?_⟩
-      · exact hsub hx
-      · intro c; exact hstuck v hsat (c v (hsat ⟨x, hx⟩))
-    · intro x; exact (congrFun (hle.form x (hS _ x.property)) _).mpr (hsat x)
-    · refine le_trans ?_ hstuck; intro u hu x
-      exact (congrFun (hle.form _ (hS _ x.property)) _).mp (hu x)
-    · intro T hST hT ⟨u, hu⟩; refine hmax T hST ?_ ?_
-      · exact le_trans hT (extens_monotone hle)
-      · use u; intro x hx; refine (congrFun (hle.form _ ?_) _).mp (hu _ hx)
-        exact extens_subset_nodes _ (hT hx)
-    · ext1 u; refine forall_congr fun x ↦ ?_
-      exact congrFun (hle.form x (hS _ x.property)) _
-
-lemma branches_monotone : @Monotone (Lpofin l) _ _ _ branches := by
-  unfold branches; intro α β hle; simp; exact branches_set_monotone hle
-
-lemma branches_not_mutually_sat {α : Lpofin l} {φ ψ : Form Node}
-    (hφ : φ ∈ α.branches) (hψ : ψ ∈ α.branches) (hneq : φ ≠ ψ) :
-    ∀ v, ¬ (φ v ∧ ψ v) := by
-  intro v ⟨h₁, h₂⟩
-  rcases (Set.Finite.mem_toFinset _).mp hφ with ⟨S, ⟨_, hsub, _, _, hmax⟩, rfl⟩
-  rcases (Set.Finite.mem_toFinset _).mp hψ with ⟨T, ⟨_, hsub', _, _, hmax'⟩, rfl⟩
-  refine hmax (S ∪ T) ⟨Finset.subset_union_left, ?_⟩ ?_ ?_
-  · intro h; apply hneq; refine congrArg _ ?_; ext x; constructor
-    · intro hx; by_contra ht; refine hmax' (insert x T) ?_ ?_ ?_
-      · exact Finset.ssubset_insert ht
-      · intro y hy; rcases Finset.mem_insert.mp hy with rfl | hy
-        · exact hsub hx
-        · exact hsub' hy
-      · use v; intro y hy; rcases Finset.mem_insert.mp hy with rfl | hy
-        · exact h₁ ⟨y, hx⟩
-        · exact h₂ ⟨y, hy⟩
-    · intro hx; exact h (Finset.subset_union_right hx)
-  · intro x hx; rcases Finset.mem_union.mp hx with hx | hx
-    · exact hsub hx
-    · exact hsub' hx
-  · use v; intro x hx; rcases Finset.mem_union.mp hx with hx | hx
-    · exact h₁ ⟨x, hx⟩
-    · exact h₂ ⟨x, hx⟩
 
 def CopyFn (α β : Lpofin l) : Type :=
   { f : ↑α.branches → Lpofin l //
@@ -188,13 +14,14 @@ def CopyFn (α β : Lpofin l) : Type :=
   }
 instance {α β : Lpofin l} : FunLike (CopyFn α β) ↑α.branches (Lpofin l) where
   coe := Subtype.val
-  coe_injective' _ _ h := Subtype.ext h
+  coe_injective _ _ h := Subtype.ext h
 
 def CopyFn_extends {α α' β β' : Lpofin l}
     (hle : α ≤ α') (f : CopyFn α β) (g : CopyFn α' β') :=
   ∀ φ : ↑α.branches, f φ ≤ g ⟨φ.val, branches_monotone hle φ.property⟩
 
-noncomputable def seq_base [DCPO l] (α β : Lpofin l) (f : CopyFn α β) : Lpo_base l := {
+open Classical in
+noncomputable def seq_base (α β : Lpofin l) (f : CopyFn α β) : Lpo_base l := {
   nodes := α.nodes ∪ ⋃ φ : ↑α.branches, (f φ).nodes
   rel x y :=
     α.rel x y ∨
@@ -206,7 +33,8 @@ noncomputable def seq_base [DCPO l] (α β : Lpofin l) (f : CopyFn α β) : Lpo_
       (f hx.choose).lab x
     else
       α.lab x
-  form x := if x ∈ α.nodes then α.form x else Form.sOr fun φ : ↑α.branches ↦ ((f φ).form x).and φ.val
+  form x :=
+    if x ∈ α.nodes then α.form x else Form.sOr fun φ : ↑α.branches ↦ ((f φ).form x).and φ.val
 }
 
 lemma branch_implies_node {α : Lpofin l} {x : Node} :
@@ -216,12 +44,12 @@ lemma branch_implies_node {α : Lpofin l} {x : Node} :
   refine (α.val.property.form_dom x).mp ?_
   rcases hsat with ⟨v, hv⟩; use v; exact hle v ((congrFun heq _).mp hv)
 
-lemma seq_nodes_finite [DCPO l] {α β : Lpofin l} {f : CopyFn α β} :
+lemma seq_nodes_finite {α β : Lpofin l} {f : CopyFn α β} :
     (seq_base α β f).nodes.Finite := by
   refine Set.finite_union.mpr ⟨α.property, ?_⟩
   refine Set.finite_iUnion ?_; intro φ; exact (f φ).property
 
-lemma seq_rel_valid [DCPO l] {α β : Lpofin l} {f : CopyFn α β} :
+lemma seq_rel_valid {α β : Lpofin l} {f : CopyFn α β} :
     (seq_base α β f).rel.IsCausalityRel (seq_base α β f).nodes := by
   have h₁ := α.val.property
   have h₂ φ := (f φ).val.property
@@ -301,8 +129,8 @@ lemma seq_rel_valid [DCPO l] {α β : Lpofin l} {f : CopyFn α β} :
       · have hy := extens_subset_nodes _ (hext hy)
         exact (α.val.property.form _ hx).2 _ (hroot _ hy heq) _ this
 
-lemma seq_valid [DCPO l] (α β : Lpofin l) (f : CopyFn α β) :
-    is_valid_lpo (seq_base α β f) := by
+lemma seq_valid(α β : Lpofin l) (f : CopyFn α β) :
+    IsValidLpo (seq_base α β f) := by
   constructor
   -- Rel Domain
   · intro x y hrel; cases hrel with
@@ -324,7 +152,7 @@ lemma seq_valid [DCPO l] (α β : Lpofin l) (f : CopyFn α β) :
     rcases hx with ⟨hx, hx'⟩
     simp only [seq_base, Subtype.exists]
     refine (dif_neg ?_).trans (α.val.property.lab_dom _ hx)
-    intro ⟨φ, hφ, hx⟩; exact hx' _ hφ hx
+    intro ⟨⟨φ, hφ⟩, hx⟩; exact hx' _ hφ hx
   -- Rel Properties
   · exact seq_rel_valid
   -- Bot Successors
@@ -458,7 +286,7 @@ lemma seq_valid [DCPO l] (α β : Lpofin l) (f : CopyFn α β) :
         have ⟨s, ⟨_, _, ⟨v, hsat⟩, _⟩, heq⟩ := (Set.Finite.mem_toFinset _).mp φ.property
         rw [← heq] at hform; exact (α.val.property.form_dom _).mp ⟨_, hform _ hsat⟩
 
-noncomputable def seq [DCPO l] (α β : Lpofin l) (f : CopyFn α β) : Lpofin l := {
+noncomputable def seq (α β : Lpofin l) (f : CopyFn α β) : Lpofin l := {
   val := {
     val := seq_base α β f
     property := seq_valid α β f
@@ -466,7 +294,8 @@ noncomputable def seq [DCPO l] (α β : Lpofin l) (f : CopyFn α β) : Lpofin l 
   property := seq_nodes_finite
 }
 
-lemma seq_monotone [DCPO l] {α α' β β' : Lpofin l} {f : CopyFn α β} {g : CopyFn α' β'}
+open Classical in
+lemma seq_monotone {α α' β β' : Lpofin l} {f : CopyFn α β} {g : CopyFn α' β'}
     (hle₁ : α ≤ α') (hext : CopyFn_extends hle₁ f g) :
     seq α β f ≤ seq α' β' g := by
   constructor
@@ -661,440 +490,6 @@ lemma seq_monotone [DCPO l] {α α' β β' : Lpofin l} {f : CopyFn α β} {g : C
           have := Finset.mem_filter.mpr.mt this; simp only [not_and, Decidable.not_not] at this
           have := this ((Set.Finite.mem_toFinset _).mpr (hle₁.nodes hz.1))
           exact this _ ((congrFun (hle₁.form _ hz.1) _).mp hform)
-
-
-namespace Equiv
-
-noncomputable def union {α : Type} {X X' Y Y' : Set α} (e₁ : X ≃ Y) (e₂ : X' ≃ Y')
-    (h₁ : Disjoint X X') (h₂ : Disjoint Y Y') :
-    ↑(X ∪ X') ≃ ↑(Y ∪ Y') :=
-  (Equiv.Set.union h₁).trans
-    ((e₁.sumCongr e₂).trans (Equiv.Set.union h₂).symm)
-
-lemma union_symm {α : Type} {X X' Y Y' : Set α} {e₁ : X ≃ Y} {e₂ : X' ≃ Y'}
-    {h₁ : Disjoint X X'} {h₂ : Disjoint Y Y'} :
-    (union e₁ e₂ h₁ h₂).symm = union e₁.symm e₂.symm h₂ h₁ := by
-  unfold union; ext1 x
-  simp only [Equiv.symm_trans_apply, Equiv.sumCongr_symm, Equiv.symm_symm,
-    Equiv.sumCongr_apply, Equiv.trans_apply]
-
-lemma union_apply_left {α : Type} {X X' Y Y' : Set α} {e₁ : X ≃ Y} {e₂ : X' ≃ Y'}
-    {h₁ : Disjoint X X'} {h₂ : Disjoint Y Y'} {x : α} (hx : x ∈ X) :
-    (union e₁ e₂ h₁ h₂ ⟨x, Set.subset_union_left hx⟩).val = (e₁ ⟨x, hx⟩).val := by
-  simp only [union, Equiv.trans_apply, Equiv.sumCongr_apply]
-  conv => arg 1; arg 1; arg 2; arg 3; exact Equiv.Set.union_apply_left _ hx
-  simp only [Sum.map_inl, Equiv.Set.union_symm_apply_left, Set.subset_union_left, Set.coe_inclusion]
-
-lemma union_apply_right {α : Type} {X X' Y Y' : Set α} {e₁ : X ≃ Y} {e₂ : X' ≃ Y'}
-    {h₁ : Disjoint X X'} {h₂ : Disjoint Y Y'} {x : α} (hx : x ∈ X') :
-    (union e₁ e₂ h₁ h₂ ⟨x, Set.subset_union_right hx⟩).val = (e₂ ⟨x, hx⟩).val := by
-  simp only [union, Equiv.trans_apply, Equiv.sumCongr_apply]
-  conv => arg 1; arg 1; arg 2; arg 3; exact Equiv.Set.union_apply_right _ hx
-  simp only [Sum.map_inr, Equiv.Set.union_symm_apply_right, Set.subset_union_right,
-    Set.coe_inclusion]
-
-lemma union_symm_apply_left {α : Type} {X X' Y Y' : Set α} {e₁ : X ≃ Y} {e₂ : X' ≃ Y'}
-    {h₁ : Disjoint X X'} {h₂ : Disjoint Y Y'} {y : α} (hy : y ∈ Y) :
-    ((union e₁ e₂ h₁ h₂).symm ⟨y, Set.subset_union_left hy⟩).val = (e₁.symm ⟨y, hy⟩).val := by
-  rw [union_symm, union_apply_left]
-
-lemma union_symm_apply_right {α : Type} {X X' Y Y' : Set α} {e₁ : X ≃ Y} {e₂ : X' ≃ Y'}
-    {h₁ : Disjoint X X'} {h₂ : Disjoint Y Y'} {y : α} (hy : y ∈ Y') :
-    ((union e₁ e₂ h₁ h₂).symm ⟨y, Set.subset_union_right hy⟩).val = (e₂.symm ⟨y, hy⟩).val := by
-  rw [union_symm, union_apply_right]
-
-lemma mem_union_left {α : Type} {X X' Y Y' : Set α} {e₁ : X ≃ Y} {e₂ : X' ≃ Y'}
-    {h₁ : Disjoint X X'} {h₂ : Disjoint Y Y'} {x}
-    (hx : (union e₁ e₂ h₁ h₂ x).val ∈ Y) : x.val ∈ X := by
-  have := @union_symm_apply_left _ _ _ _ _ e₁ e₂ h₁ h₂ _ hx
-  simp only [Subtype.coe_eta, Equiv.symm_apply_apply] at this; rw [this]; exact Subtype.coe_prop _
-
-lemma mem_union_right {α : Type} {X X' Y Y' : Set α} {e₁ : X ≃ Y} {e₂ : X' ≃ Y'}
-    {h₁ : Disjoint X X'} {h₂ : Disjoint Y Y'} {x}
-    (hx : (union e₁ e₂ h₁ h₂ x).val ∈ Y') : x.val ∈ X' := by
-  have := @union_symm_apply_right _ _ _ _ _ e₁ e₂ h₁ h₂ _ hx
-  simp only [Subtype.coe_eta, Equiv.symm_apply_apply] at this; rw [this]; exact Subtype.coe_prop _
-
-lemma mem_union_symm_left {α : Type} {X X' Y Y' : Set α} {e₁ : X ≃ Y} {e₂ : X' ≃ Y'}
-    {h₁ : Disjoint X X'} {h₂ : Disjoint Y Y'} {y}
-    (hy : ((union e₁ e₂ h₁ h₂).symm y).val ∈ X) : y.val ∈ Y := by
-  have := @union_apply_left _ _ _ _ _ e₁ e₂ h₁ h₂ _ hy
-  simp only [Subtype.coe_eta, Equiv.apply_symm_apply] at this; rw [this]; exact Subtype.coe_prop _
-
-lemma mem_union_symm_right {α : Type} {X X' Y Y' : Set α} {e₁ : X ≃ Y} {e₂ : X' ≃ Y'}
-    {h₁ : Disjoint X X'} {h₂ : Disjoint Y Y'} {y}
-    (hy : ((union e₁ e₂ h₁ h₂).symm y).val ∈ X') : y.val ∈ Y' := by
-  have := @union_apply_right _ _ _ _ _ e₁ e₂ h₁ h₂ _ hy
-  simp only [Subtype.coe_eta, Equiv.apply_symm_apply] at this; rw [this]; exact Subtype.coe_prop _
-
-noncomputable def sigma_iUnion {α β : Type} {f : α → Set β}
-    (h : ∀ x y, x ≠ y → Disjoint (f x) (f y)) :
-    Sigma (fun x ↦ ↑(f x)) ≃ ↑(Set.iUnion f) := {
-  toFun x := ⟨x.snd.val, Set.mem_iUnion.mpr ⟨x.fst, x.snd.property⟩⟩
-  invFun x := by
-    have := Set.mem_iUnion.mp x.property
-    exact Sigma.mk this.choose ⟨x.val, this.choose_spec⟩
-  left_inv x := by
-    ext <;> simp only
-    by_contra hc
-    let p i := x.snd.val ∈ f i
-    exact Set.disjoint_left.mp (h _ _ hc) (Exists.choose_spec (p := p) _) x.snd.property
-  right_inv x := by simp only [Subtype.coe_eta]
-}
-
-noncomputable def iUnion {ι κ α : Type} {f : ι → Set α} {g : κ → Set α}
-    (h₁ : ∀ x y, x ≠ y → Disjoint (f x) (f y))
-    (h₂ : ∀ x y, x ≠ y → Disjoint (g x) (g y))
-    (e : ι ≃ κ) (e' : (i : ι) → f i ≃ g (e i)) :
-    ↑(Set.iUnion f) ≃ ↑(Set.iUnion g) :=
-  (Equiv.sigma_iUnion h₁).symm.trans
-    ((Equiv.sigmaCongr e e').trans (Equiv.sigma_iUnion h₂))
-
-lemma iUnion_apply {ι κ α : Type} {f : ι → Set α} {g : κ → Set α}
-    {h₁ : ∀ x y, x ≠ y → Disjoint (f x) (f y)}
-    {h₂ : ∀ x y, x ≠ y → Disjoint (g x) (g y)}
-    {e : ι ≃ κ} {e' : (i : ι) → f i ≃ g (e i)}
-    {x : α} {i : ι} (hx : x ∈ f i) :
-    (iUnion h₁ h₂ e e' ⟨x, Set.subset_iUnion _ _ hx⟩).val = (e' i ⟨x, hx⟩).val := by
-  simp only [iUnion, sigma_iUnion, Equiv.sigmaCongr, Equiv.trans_apply, Equiv.coe_fn_symm_mk,
-    Equiv.sigmaCongrRight_apply, Equiv.sigmaCongrLeft_apply, Equiv.coe_fn_mk]
-  have h := Set.mem_iUnion.mp (Set.subset_iUnion _ _ hx)
-  have : h.choose = i := by
-    refine not_not.mp ((h₁ _ _).mt ?_)
-    exact Set.not_disjoint_iff.mpr ⟨x, h.choose_spec, hx⟩
-  subst this; rfl
-
-def swap_fun {ι κ α : Type} {f : ι → Set α} {g : κ → Set α}
-    (e : ι ≃ κ) (e' : (i : ι) → f i ≃ g (e i)) :
-    (k : κ) → g k ≃ f (e.symm k) :=
-  fun k ↦
-    (Equiv.setCongr (by simp only [Equiv.apply_symm_apply])).trans (e' (e.symm k)).symm
-
-lemma iUnion_symm {ι κ α : Type} {f : ι → Set α} {g : κ → Set α}
-    {h₁ : ∀ x y, x ≠ y → Disjoint (f x) (f y)}
-    {h₂ : ∀ x y, x ≠ y → Disjoint (g x) (g y)}
-    {e : ι ≃ κ} {e' : (i : ι) → f i ≃ g (e i)} :
-    (iUnion h₁ h₂ e e').symm =
-    iUnion h₂ h₁ e.symm (swap_fun e e') := by
-  ext1 x; unfold swap_fun
-  simp only [iUnion, sigma_iUnion, Equiv.sigmaCongr, Equiv.sigmaCongrRight, Equiv.sigmaCongrLeft,
-    Equiv.symm_trans_apply, Equiv.symm_symm, Equiv.coe_fn_symm_mk, Equiv.coe_fn_mk,
-    Equiv.trans_apply, Equiv.setCongr_apply, Equiv.setCongr_symm_apply, Subtype.mk.injEq]
-  refine congrArg _ (congrArg _ ?_)
-  ext; grind only
-
-lemma iUnion_symm_apply {ι κ α : Type} {f : ι → Set α} {g : κ → Set α}
-    {h₁ : ∀ x y, x ≠ y → Disjoint (f x) (f y)}
-    {h₂ : ∀ x y, x ≠ y → Disjoint (g x) (g y)}
-    {e : ι ≃ κ} {e' : (i : ι) → f i ≃ g (e i)}
-    {y : α} {k : κ} (hy : y ∈ g k) :
-    ((iUnion h₁ h₂ e e').symm ⟨y, Set.subset_iUnion _ _ hy⟩).val =
-    ((e' (e.symm k)).symm ⟨y, by simpa only [Equiv.apply_symm_apply]⟩).val := by
-  rw [iUnion_symm]; refine (iUnion_apply hy).trans ?_
-  simp only [swap_fun, Equiv.trans_apply, Equiv.setCongr_apply]
-
-lemma iUnion_symm_apply' {ι κ α : Type} {f : ι → Set α} {g : κ → Set α}
-    {h₁ : ∀ x y, x ≠ y → Disjoint (f x) (f y)}
-    {h₂ : ∀ x y, x ≠ y → Disjoint (g x) (g y)}
-    {e : ι ≃ κ} {e' : (i : ι) → f i ≃ g (e i)}
-    {y : α} {i : ι} (hy : y ∈ g (e i)) :
-    ((iUnion h₁ h₂ e e').symm ⟨y, Set.subset_iUnion _ _ hy⟩).val =
-    ((e' i).symm ⟨y, by simpa only [Equiv.apply_symm_apply]⟩).val := by
-  rw [iUnion_symm]; refine (iUnion_apply hy).trans ?_
-  simp [swap_fun]; sorry
-
-lemma mem_iUnion {ι κ α : Type} {f : ι → Set α} {g : κ → Set α}
-    {h₁ : ∀ x y, x ≠ y → Disjoint (f x) (f y)}
-    {h₂ : ∀ x y, x ≠ y → Disjoint (g x) (g y)}
-    {e : ι ≃ κ} {e' : (i : ι) → f i ≃ g (e i)}
-    {x : ↑(⋃ i, f i)} {k : κ} (h : (iUnion h₁ h₂ e e' x).val ∈ g k) :
-    x.val ∈ f (e.symm k) := by
-  have := @iUnion_symm_apply _ _ _ _ _ h₁ h₂ e e' _ _ h
-  simp only [Subtype.coe_eta, Equiv.symm_apply_apply] at this
-  rw [this]; exact Subtype.coe_prop _
-
-lemma mem_iUnion_symm {ι κ α : Type} {f : ι → Set α} {g : κ → Set α}
-    {h₁ : ∀ x y, x ≠ y → Disjoint (f x) (f y)}
-    {h₂ : ∀ x y, x ≠ y → Disjoint (g x) (g y)}
-    {e : ι ≃ κ} {e' : (i : ι) → f i ≃ g (e i)}
-    {y : ↑(⋃ k, g k)} {i : ι} (h : ((iUnion h₁ h₂ e e').symm y).val ∈ f i) :
-    y.val ∈ g (e i) := by
-  have := @iUnion_apply _ _ _ _ _ h₁ h₂ e e' _ _ h
-  simp only [Subtype.coe_eta, Equiv.apply_symm_apply] at this
-  rw [this]; exact Subtype.coe_prop _
-
-end Equiv
-
-lemma branches_permute {α α' : Lpofin l} {e : α.nodes ≃ α'.nodes}
-    (h : α.permute e = α') :
-    ∀ φ ∈ α.branches, φ.permute e ∈ α'.branches := by
-  intro φ hφ
-  obtain ⟨s, ⟨hne, hsub, ⟨v, hsat⟩, hstk, hmax⟩, rfl⟩ := (Set.Finite.mem_toFinset _).mp hφ
-  let t := s.attach.image
-    (fun x : ↑s ↦ (e ⟨x.val, extens_subset_nodes _ (hsub x.property)⟩).val)
-  refine (Set.Finite.mem_toFinset _).mpr ⟨t, ⟨?_, ?_, ?_, ?_, ?_⟩, ?_⟩ <;> subst t
-  · refine Finset.Nonempty.image (Finset.univ_nonempty_iff.mpr ?_) _
-    exact hne.coe_sort
-  · conv => rhs; rw [← h]
-    intro x hx; obtain ⟨⟨y, hy⟩, _, rfl⟩ := Finset.mem_image.mp hx
-    simp only [extens, Finset.mem_filter]; constructor
-    · refine (Set.Finite.mem_toFinset _).mpr ?_; exact Subtype.coe_prop _
-    · intro hc
-      have := hsub hy; simp [extens] at this; have ⟨hy', h'⟩ := this; apply h'
-      have hy' := (Set.Finite.mem_toFinset _).mp hy'; intro v hform
-      have ⟨⟨z, hz, hbot⟩, _, hform'⟩ := hc (Form.image v e) ((Lpo.permute_form_sat_iff hy').mp hform)
-      refine ⟨⟨(e.symm ⟨_, hz⟩).val, Subtype.coe_prop _, ?_⟩, ?_⟩
-      · refine Eq.trans ?_ hbot; exact (if_pos hz).symm
-      · refine (Lpo.permute_form_sat_iff (Subtype.coe_prop _) (e := e)).mpr ?_
-        conv => arg 2; arg 1; exact e.apply_symm_apply _
-        exact ⟨hz, hform'⟩
-  · use Form.image v e; intro ⟨x, hx⟩; obtain ⟨⟨y, hy⟩, _, rfl⟩ := Finset.mem_image.mp hx
-    conv => simp only; arg 1; exact h.symm
-    refine (Lpo.permute_form_sat_iff _).mp (hsat ⟨_, hy⟩)
-  · intro v hv ⟨⟨z, hz, hbot⟩, hform⟩
-    refine hstk (Form.image v e.symm) ?_ ?_
-    · intro ⟨x, hx⟩; refine ((Lpo.permute_form_sat_iff ?_ (e := e)).mpr ?_)
-      · exact extens_subset_nodes _ (hsub hx)
-      · conv => arg 3; arg 2; exact e.symm_symm.symm
-        conv => arg 3; exact Form.image_inv v e.symm
-        refine Lpo.form_inter_nodes_sat_iff.mp ?_
-        conv at hv => arg 1; exact h.symm
-        refine hv ⟨(e ⟨x, _⟩).val, ?_⟩
-        exact Finset.mem_image.mpr ⟨⟨x, hx⟩, Finset.mem_attach _ _, rfl⟩
-    · refine ⟨⟨(e.symm ⟨z, hz⟩).val, Subtype.coe_prop _, ?_⟩, ?_⟩
-      · rw [← h] at hbot; simp only [Lpo.lab, permute, Lpo.permute, dite_eq_right_iff] at hbot
-        exact hbot hz
-      · simp only
-        refine (Lpo.permute_form_sat_iff (Subtype.coe_prop _) (e := e)).mpr ?_
-        conv => arg 3; exact Form.image_inv v e.symm
-        refine Lpo.form_inter_nodes_sat_iff.mp ?_
-        conv => arg 2; simp only [Subtype.coe_eta]; arg 1; exact e.apply_symm_apply _
-        conv at hform => simp only; arg 1; exact h.symm
-        exact hform
-  · intro t ⟨hst, hnts⟩ hex ⟨v, hform⟩
-    refine hmax (t.attach.image fun y ↦ (e.symm ⟨y.val, ?_⟩).val) ?_ ?_ ?_
-    · exact extens_subset_nodes _ (hex y.property)
-    · constructor
-      · intro x hx; refine Finset.mem_image.mpr ⟨⟨e ⟨x, ?_⟩, ?_⟩, Finset.mem_attach _ _, ?_⟩
-        · exact extens_subset_nodes _ (hsub hx)
-        · exact hst (Finset.mem_image.mpr ⟨⟨x, hx⟩, Finset.mem_attach _ _, rfl⟩)
-        · simp only [Subtype.coe_eta, Equiv.symm_apply_apply]
-      · intro hc; apply hnts; intro x hx
-        refine Finset.mem_image.mpr ⟨⟨(e.symm ⟨x, ?_⟩).val, ?_⟩, Finset.mem_attach _ _, ?_⟩
-        · exact extens_subset_nodes _ (hex hx)
-        · exact hc (Finset.mem_image.mpr ⟨⟨x, hx⟩, Finset.mem_attach _ _, rfl⟩)
-        · simp only [Subtype.coe_eta, Equiv.apply_symm_apply]
-    · intro x hx; simp only [extens, Finset.mem_image, Finset.mem_attach, true_and, Finset.mem_filter] at *
-      obtain ⟨y, rfl⟩ := hx; constructor
-      · exact (Set.Finite.mem_toFinset _).mpr (Subtype.coe_prop _)
-      · intro hc; have := hex y.property
-        simp only [extens, nodes_finset, Finset.mem_filter, Set.Finite.mem_toFinset] at this
-        apply this.2; intro v hform
-        rw [← h] at hform; simp only [Lpofin.permute, form, Lpo.permute, Lpo.form] at hform
-        have ⟨hy, hform⟩ := hform
-        have ⟨⟨z, hz, hbot⟩, hform⟩ := hc _ hform
-        refine ⟨⟨(e ⟨_, hz⟩).val, Subtype.coe_prop _, ?_⟩, ?_⟩
-        · conv => arg 1; arg 1; arg 1; exact h.symm
-          simp only [Lpofin.permute, Lpo.permute, Lpo.lab]
-          refine (dif_pos (Subtype.coe_prop _)).trans ?_
-          conv => lhs; arg 2; simp only [Subtype.coe_eta]; arg 1; exact e.symm_apply_apply _
-          exact hbot
-        · simp only [← h]
-          refine Lpo.form_inter_nodes_sat_iff.mpr ?_
-          conv => arg 3; exact (Form.image_inv _ e.symm).symm
-          conv => arg 3; arg 2; exact e.symm_symm
-          exact (Lpo.permute_form_sat_iff _).mp hform
-    · refine ⟨Form.image v e.symm, ?_⟩; intro x hx
-      obtain ⟨y, _, rfl⟩ := Finset.mem_image.mp hx
-      refine (Lpo.permute_form_sat_iff (Subtype.coe_prop _) (e := e)).mpr ?_
-      conv => arg 2; simp only [Subtype.coe_eta]; arg 1; exact e.apply_symm_apply _
-      conv => arg 3; exact Form.image_inv _ _
-      refine Lpo.form_inter_nodes_sat_iff.mp ?_
-      have := hform _ y.property; rw [← h] at this; exact this
-  · conv => lhs; arg 1; rw [← h]
-    simp only [conj]; unfold Form.permute; ext v; constructor
-    · intro hform x
-      have :=
-        hform
-          ⟨(e ⟨x.val, extens_subset_nodes _ (hsub x.property)⟩).val,
-            Finset.mem_image.mpr ⟨x, Finset.mem_attach _ _, rfl⟩⟩
-      simp only [form, Lpo.form, permute, Lpo.permute, Form.permute, Subtype.coe_eta,
-        Subtype.coe_prop, exists_const] at this
-      conv at this => arg 2; arg 1; exact Equiv.symm_apply_apply _ _
-      exact this
-    · intro hform x
-      have ⟨y, _, heq⟩ := Finset.mem_image.mp x.property; rw [← heq]
-      have := hform y
-      simp only [form, Lpo.form, permute, Lpo.permute, Form.permute, Subtype.coe_eta,
-        Subtype.coe_prop, exists_const]
-      conv => arg 2; arg 1; exact Equiv.symm_apply_apply _ _
-      exact this
-
-def branches_equiv [PartialOrder l] [OrderBot l] {α α' : Lpofin l} {e : α.nodes ≃ α'.nodes}
-    (h : α.permute e = α') :
-    α.branches ≃ α'.branches := {
-  toFun φ := ⟨φ.val.permute e, branches_permute h _ φ.property⟩
-  invFun φ := ⟨φ.val.permute e.symm, by {
-    refine branches_permute ?_ _ φ.property
-    refine Subtype.ext ?_; symm; refine (Lpo.permute_symm ?_)
-    conv => rhs; arg 1; exact h.symm
-    rfl
-  }⟩
-  left_inv := by
-    intro ⟨φ, hφ⟩
-    unfold Form.permute; ext1; ext1 v; simp only [Equiv.symm_symm, Form.image]
-    obtain ⟨s, ⟨_, hsub, _⟩, rfl⟩:= (Set.Finite.mem_toFinset _).mp hφ
-    have h (x : ↑s) := (α.val.property.form _ (extens_subset_nodes _ (hsub x.property))).1
-    refine Form.DependsOn.sAnd h _ _ ?_
-    refine Set.disjoint_left.mpr ?_; intro x hx hx'
-    have ⟨y, hrel⟩ := Set.mem_iUnion.mp hx'
-    rcases Set.mem_symmDiff.mp hx with ⟨⟨z, rfl, w, heq, hw⟩, hv⟩ | ⟨hv, h⟩
-    · apply hv; rw [← Subtype.val_injective heq]; simpa only [Equiv.symm_apply_apply]
-    · have hx := (α.val.property.rel_dom hrel).1
-      refine h ⟨e ⟨x, hx⟩, ?_, ⟨x, hx⟩, rfl, hv⟩
-      simp only [Equiv.symm_apply_apply]
-  right_inv := by
-    intro ⟨φ, hφ⟩
-    unfold Form.permute; ext1; ext1 v; simp only [Form.image, Equiv.symm_symm, Subtype.exists,
-      exists_and_right, Set.mem_setOf_eq, ↓existsAndEq, Subtype.coe_eta, Equiv.apply_symm_apply,
-      Subtype.coe_prop, exists_const, true_and, exists_prop]
-    obtain ⟨s, ⟨_, hsub, _⟩, rfl⟩:= (Set.Finite.mem_toFinset _).mp hφ
-    have h (x : ↑s) := (α'.val.property.form _ (extens_subset_nodes _ (hsub x.property))).1
-    refine Form.DependsOn.sAnd h _ _ ?_
-    refine Set.disjoint_left.mpr ?_; intro x hx hx'
-    have ⟨y, hrel⟩ := Set.mem_iUnion.mp hx'
-    rcases Set.mem_symmDiff.mp hx with ⟨⟨_, h⟩, h'⟩ | ⟨hv, h⟩
-    · exact h' h
-    · refine h ⟨⟨?_, True.intro⟩, hv⟩; exact (α'.val.property.rel_dom hrel).1
-}
-
-lemma seq_isomorphic [DCPO l] [OrderBot l] {α α' β β' : Lpofin l} {f : CopyFn α β} {g : CopyFn α' β'}
-    (hα : α ≈ α') (hβ : β ≈ β') : seq α β f ≈ seq α' β' g := by
-  have ⟨e, he⟩ := hα
-  have eb := branches_equiv (Subtype.ext he)
-  have (φ : ↑α.branches) :
-      ∃ e : ((f φ).nodes ≃ (g (eb φ)).nodes), (f φ).permute e = (g (eb φ)) := by
-    have ⟨ef, hf⟩ := (f.property φ).1
-    have ⟨eg, hg⟩ := (g.property (eb φ)).1
-    have ⟨eβ, h⟩ := hβ
-    refine ⟨ef.trans (eβ.trans eg.symm), ?_⟩
-    unfold Lpofin.permute; refine Subtype.ext ?_; simp only
-    refine Lpo.permute_trans.symm.trans ?_
-    refine Lpo.permute_trans.symm.trans ?_
-    symm; refine Lpo.permute_symm (hg.trans (h.symm.trans ?_))
-    refine Lpo.permute_congr _ _ hf.symm ?_
-    intro x; rfl
-  choose eφ h using this
-  let e' := Equiv.iUnion
-    (fun φ ↦ (f.property φ).2.2)
-    (fun φ ↦ (g.property φ).2.2)
-    eb eφ
-  refine ⟨Equiv.union e e' ?_ ?_ , ?_⟩
-  · refine Set.disjoint_left.mpr ?_; intro x hx hx'
-    have ⟨φ, hx'⟩ := Set.mem_iUnion.mp hx'
-    exact Set.disjoint_left.mp (f.property φ).2.1 hx hx'
-  · refine Set.disjoint_left.mpr ?_; intro x hx hx'
-    have ⟨φ, hx'⟩ := Set.mem_iUnion.mp hx'
-    exact Set.disjoint_left.mp (g.property φ).2.1 hx hx'
-  · ext1
-    · rfl
-    · ext x y
-      by_cases hx : x ∈ (α'.seq β' g).nodes
-      · by_cases hy : y ∈ (α'.seq β' g).nodes
-        · simp only [seq, seq_base, Lpo.permute, Lpo.nodes, Lpo.rel]
-          unfold Rel.permute
-          refine Iff.trans ⟨fun h ↦ h.2.2, fun h ↦ ⟨hx, hy, h⟩⟩ ?_
-          refine or_congr ?_ ?_
-          · unfold Lpofin.rel; rw [← he]
-            simp only [Lpo.permute, Lpo.rel, Rel.permute]
-            constructor
-            · intro hrel; have ⟨hx', hy'⟩ := (α.val.property.rel_dom hrel)
-              have hx := Equiv.mem_union_symm_left hx'
-              have hy := Equiv.mem_union_symm_left hy'
-              refine ⟨hx, hy, ?_⟩
-              rw [Equiv.union_symm_apply_left hx, Equiv.union_symm_apply_left hy] at hrel
-              exact hrel
-            · intro ⟨hx', hy', hrel⟩
-              refine (congrArg₂ α.rel ?_ ?_).mpr hrel
-              · exact Equiv.union_symm_apply_left hx'
-              · exact Equiv.union_symm_apply_left hy'
-          · refine eb.exists_congr ?_; intro φ
-            rw [← h φ]
-            simp only [Lpofin.permute, Lpo.permute, rel, Lpo.rel, nodes, Lpo.nodes, Rel.permute]
-            refine or_congr ?_ ?_
-            · constructor
-              · intro hrel
-                have ⟨hx', hy'⟩ := (f φ).val.property.rel_dom hrel
-                have hx'' := Equiv.mem_union_symm_right (Set.mem_iUnion.mpr ⟨_, hx'⟩)
-                have hy'' := Equiv.mem_union_symm_right (Set.mem_iUnion.mpr ⟨_, hy'⟩)
-                conv at hx' => arg 2; exact Equiv.union_symm_apply_right hx''
-                conv at hy' => arg 2; exact Equiv.union_symm_apply_right hy''
-                unfold e' at hx'
-                have hx := Equiv.mem_iUnion_symm (e := eb) hx'
-                have hy := Equiv.mem_iUnion_symm (e := eb) hy'
-                refine ⟨hx, hy, (congrArg₂ _ ?_ ?_).mp hrel⟩; all_goals {
-                  refine (Equiv.union_symm_apply_right ?_).trans ?_
-                  · assumption
-                  · exact Equiv.iUnion_symm_apply' _
-                }
-              · intro ⟨hx', hy', hrel⟩
-                refine (congrArg₂ _ ?_ ?_).mpr hrel; all_goals {
-                  refine (Equiv.union_symm_apply_right ?_).trans ?_
-                  · refine Set.mem_iUnion.mpr ⟨eb φ, ?_⟩; assumption
-                  · exact Equiv.iUnion_symm_apply' _
-                }
-            · refine and_congr ?_ ?_
-              · sorry
-              · sorry
-        · constructor
-          · intro ⟨_, hy', _⟩; exfalso; exact hy hy'
-          · intro hrel; exfalso; exact hy ((seq _ _ _).val.property.rel_dom hrel).2
-      · constructor
-        · intro ⟨hx', _⟩; exfalso; exact hx hx'
-        · intro hrel; exfalso; exact hx ((seq _ _ _).val.property.rel_dom hrel).1
-
-
-
-      constructor
-      · rintro ⟨hx, hy, hrel | ⟨φ, hrel | ⟨hform, hj⟩⟩⟩
-        · left; unfold Lpofin.rel; rw [← he]; simp only [Lpo.permute, Lpo.rel, Rel.permute]
-          have ⟨hx', hy'⟩ := (α.val.property.rel_dom hrel)
-          have hx := Equiv.mem_union_symm_left hx'
-          have hy := Equiv.mem_union_symm_left hy'
-          refine ⟨hx, hy, ?_⟩
-          rw [Equiv.union_symm_apply_left hx, Equiv.union_symm_apply_left hy] at hrel
-          exact hrel
-        · right; use eb φ; left
-          have ⟨hx', hy'⟩ := (f φ).val.property.rel_dom hrel
-          rw [← h φ]; simp only [Lpofin.permute, rel, Lpo.permute, Lpo.rel, Rel.permute]
-          sorry
-        · sorry
-      · intro h; sorry
-    · simp only [seq, seq_base, Lpo.permute, Lpo.lab, Lpo.nodes]
-      ext x; by_cases hx : x ∈ α'.nodes ∪ ⋃ φ, (g φ).nodes
-      · conv => lhs; exact dif_pos hx
-        by_cases hx' : ∃ φ, x ∈ (g φ).nodes
-        · conv => rhs; exact dif_pos hx'
-          have ⟨φ, hx'⟩ := hx'
-          refine (dif_pos ?_).trans ?_
-          · use eb.symm φ; sorry
-          · conv => rhs; arg 1; arg 2; exact (eb.apply_symm_apply _).symm
-            conv => rhs; arg 1; exact (h _).symm
-            simp only [permute, lab, Lpo.permute, Lpo.lab]
-            sorry
-      · conv => lhs; exact dif_neg hx
-        symm; refine (dif_neg ?_).trans ?_
-        · intro ⟨φ, hφ⟩; apply hx; right; exact Set.mem_iUnion.mpr ⟨_, hφ⟩
-        · refine α'.val.property.lab_dom _ ?_
-          intro hx'; apply hx; left; exact hx'
-    · simp only [seq, seq_base, Lpo.permute, Lpo.form, Lpo.nodes]
-      ext x v; constructor
-      · intro ⟨hx, hform⟩
-        rcases hx with hx | hx
-        · rw [if_pos hx, Lpofin.form, ← he]
-          use hx
-
-          --conv => congrFun (if_pos hx) _
 
 
 end Lpofin
