Pom/Lpo/Operations/Seq/Branches.lean
@@ -1,0 +1,182 @@
+import Pom.Lpo.Order.FinApprox
+
+namespace Lpofin
+open Classical
+
+variable {l : Type} [PartialOrder l] [OrderBot l]
+
+-- stuck is a path condition formula indicating that the execution will definitely
+-- encounter a ⊥ node
+def stuck (α : Lpofin l) : Form Node := Form.sOr fun x : ↑α.val.bots ↦ α.form x.val
+
+lemma stuck_antitone : @Antitone (Lpofin l) _ _ _ stuck := by
+  intro α β hle v ⟨⟨x, hx, hlab⟩, hform⟩
+  rcases hle.succ _ hx with hx' | ⟨y, ⟨hy, hlab'⟩, hyx⟩
+  · refine ⟨⟨x, hx', ?_⟩, ?_⟩
+    · refine le_antisymm ?_ bot_le
+      rw [← hlab]; exact hle.lab x
+    · refine (congrFun (hle.form x hx') v).mpr ?_
+      exact hform
+  · refine ⟨⟨y, hy, hlab'⟩, ?_⟩
+    refine (congrFun (hle.form _ hy) _).mpr ?_
+    refine (β.val.property.form _ (hle.nodes hy)).2 _ hyx _ ?_
+    exact hform
+
+-- A node is in the exntensible set if it is possible for it not be stuck
+noncomputable def extens (α : Lpofin l) : Finset Node :=
+  α.nodes_finset.filter fun x ↦ ¬ α.form x ≤ α.stuck
+
+lemma extens_not_bot {α : Lpofin l} {x : Node} : x ∈ α.extens → α.lab x ≠ ⊥ := by
+  intro h; simp only [extens, Finset.mem_filter] at h; intro heq; apply h.2; intro v hform
+  refine ⟨⟨x, ?_, heq⟩, hform⟩
+  exact (α.val.property.form_dom x).mp ⟨v, hform⟩
+
+lemma extens_subset_nodes {α : Lpofin l} : ∀ x ∈ α.extens, x ∈ α.nodes := by
+  intro x hx; exact (Set.Finite.mem_toFinset _).mp (Finset.mem_filter.mp hx).1
+
+lemma extens_monotone : @Monotone (Lpofin l) _ _ _ extens := by
+  intro α β hle x; simp only [extens, Finset.mem_filter, and_imp]; intro hx hstuck
+  have hx' := (Set.Finite.mem_toFinset _).mp hx
+  refine ⟨(Set.Finite.mem_toFinset _).mpr (hle.nodes hx'), fun hc ↦ ?_⟩
+  refine hstuck (fun v hform ↦ stuck_antitone hle v (hc v ?_))
+  simp only [form]; rw [← hle.form x hx']; exact hform
+
+lemma le_extens {α β : Lpofin l} (hle : α ≤ β) :
+    α.extens = β.extens.filter fun x ↦ ¬ (β.form x ≤ α.stuck) := by
+  ext x; constructor
+  · intro hx; refine Finset.mem_filter.mpr ⟨extens_monotone hle hx, ?_⟩
+    intro c; refine (Finset.mem_filter.mp hx).2 (le_trans ?_ c)
+    exact le_form hle
+  · intro hx; obtain ⟨hx, hstk⟩ := Finset.mem_filter.mp hx
+    obtain ⟨hx', _⟩ := Finset.mem_filter.mp hx
+    apply (Set.Finite.mem_toFinset _).mp at hx'
+    rcases hle.succ _  hx' with hxα | ⟨y, ⟨hy, hbot⟩, hyx⟩
+    · refine Finset.mem_filter.mpr ⟨(Set.Finite.mem_toFinset _).mpr hxα, ?_⟩
+      intro c; refine hstk (le_of_eq_of_le (Eq.symm ?_) c)
+      exact hle.form _ hxα
+    · exfalso; refine hstk (((β.val.property.form y (hle.nodes hy)).2 _ hyx).trans ?_)
+      refine le_of_eq_of_le (Eq.symm (hle.form _ hy)) ?_
+      intro v hform; exact ⟨⟨y, hy, hbot⟩, hform⟩
+
+def conj (α : Lpofin l) (S : Finset Node) : Form Node :=
+  Form.sAnd fun x : ↑S ↦ α.form x.val
+
+def branches_set (α : Lpofin l) : Set (Form Node) :=
+  α.conj ''
+  { S : Finset Node
+  | S.Nonempty ∧
+    S ⊆ α.extens ∧
+    (α.conj S).sat ∧
+    α.conj S ≤ α.stuck.not ∧
+    ∀ T, S ⊂ T → T ⊆ α.extens → ¬ Form.sat (fun v ↦ ∀ x ∈ T, α.form x v)
+  }
+
+lemma branches_finite (α : Lpofin l) : α.branches_set.Finite := by
+  refine Set.Finite.image _ ?_
+  refine Set.Finite.subset α.extens.powerset.finite_toSet ?_
+  intro s ⟨_, hsub, _⟩; simp only [Finset.coe_powerset, Set.mem_preimage, Set.mem_powerset_iff,
+    Finset.coe_subset, hsub]
+
+noncomputable def branches (α : Lpofin l) : Finset (Form Node) := α.branches_finite.toFinset
+
+lemma branches_set_monotone : @Monotone (Lpofin l) _ _ _ branches_set := by
+  rintro α β hle φ ⟨S, ⟨hne, hsub, hsat, hstuck, hmax⟩, hφ⟩; subst hφ
+  refine ⟨S, ⟨hne, ?_, ?_, ?_, ?_⟩, ?_⟩
+  · exact le_trans hsub (extens_monotone hle)
+  · rcases hsat with ⟨v, hv⟩; use v; intro x
+    refine (congrFun (hle.form x ?_) _).mp (hv x)
+    have hx' := Finset.mem_of_mem_filter _ (hsub x.property)
+    exact (Set.Finite.mem_toFinset _).mp hx'
+  · intro v hform hstuck'; refine hstuck v ?_ ?_
+    · intro x; refine (congr_fun (hle.form x ?_) v).mpr (hform x)
+      have hx' := Finset.mem_of_mem_filter _ (hsub x.property)
+      exact (Set.Finite.mem_toFinset _).mp hx'
+    · exact stuck_antitone hle v hstuck'
+  · intro T hST hT ⟨v, hc⟩; obtain ⟨x, hxT, hxS⟩ := Finset.exists_of_ssubset hST
+    have hform : α.conj S v := by
+      intro y; refine (congrFun (hle.form _ ?_) _).mpr (hc _ ?_)
+      · exact extens_subset_nodes _ (hsub y.property)
+      · exact (Finset.ssubset_def.mp hST).1 y.property
+    rcases hle.succ _ (extens_subset_nodes _ (hT hxT))
+      with hx | ⟨y, hy, hyx⟩
+    · refine hmax (insert x S) (Finset.ssubset_insert hxS) ?_ ?_
+      · refine Finset.insert_subset (Finset.mem_filter.mpr ⟨?_, ?_⟩) hsub
+        · exact (Set.Finite.mem_toFinset _).mpr hx
+        · intro c; refine hstuck v hform ?_
+          exact c v ((congrFun (hle.form _ hx) _).mpr (hc _ hxT))
+      · use v; intro y hy; rcases Finset.mem_insert.mp hy with rfl | hy'
+        · exact (congrFun (hle.form y hx) _).mpr (hc y hxT)
+        · refine (congrFun (hle.form y ?_) _).mpr (hc y ?_)
+          · exact extens_subset_nodes _ (hsub hy')
+          · exact Finset.mem_of_subset (Finset.ssubset_def.mp hST).1 hy'
+    · refine hstuck v hform ⟨⟨y, hy⟩, ?_⟩
+      refine (congrFun (hle.form _ hy.1) _).mpr ?_
+      exact (β.val.property.form _ (hle.nodes hy.1)).2 _ hyx v (hc _ hxT)
+  · ext1 v; refine forall_congr fun x ↦ ?_; ext; constructor
+    · intro h; refine (congr_fun (hle.form x ?_) v).mpr h
+      have hx' := Finset.mem_of_mem_filter _ (hsub x.property)
+      exact (Set.Finite.mem_toFinset _).mp hx'
+    · intro h; refine (congr_fun (hle.form x ?_) v).mp h
+      have hx' := Finset.mem_of_mem_filter _ (hsub x.property)
+      exact (Set.Finite.mem_toFinset _).mp hx'
+
+lemma le_branches_set {α β : Lpofin l} (hle : α ≤ β) :
+    α.branches_set = { φ ∈ β.branches_set | φ ≤ α.stuck.not } := by
+  ext φ; constructor
+  · intro h; constructor
+    · exact branches_set_monotone hle h
+    · rcases h with ⟨_, ⟨_, _, _, hstuck, _⟩, rfl⟩
+      exact hstuck
+  · rintro ⟨⟨S, ⟨hne, hsub, ⟨v, hsat⟩, _, hmax⟩, rfl⟩, hstuck⟩
+    have hS x (hx : x ∈ S) : x ∈ α.nodes := by
+      have hx' := extens_subset_nodes _ (hsub hx)
+      rcases hle.succ _ hx' with hxα | ⟨y, hbot, hyx⟩
+      · exact hxα
+      · exfalso; refine forall_not_of_not_exists (hstuck v hsat) ⟨y, hbot⟩ ?_
+        refine (congrFun (hle.form y hbot.1) _).mpr ?_
+        refine (β.val.property.form y (hle.nodes hbot.1)).2 _ hyx v ?_
+        exact hsat ⟨_, hx⟩
+    refine ⟨S, ⟨hne, ?_, ⟨v, ?_⟩, ?_, ?_⟩, ?_⟩
+    · intro x hx; rw [le_extens hle]; refine Finset.mem_filter.mpr ⟨?_, ?_⟩
+      · exact hsub hx
+      · intro c; exact hstuck v hsat (c v (hsat ⟨x, hx⟩))
+    · intro x; exact (congrFun (hle.form x (hS _ x.property)) _).mpr (hsat x)
+    · refine le_trans ?_ hstuck; intro u hu x
+      exact (congrFun (hle.form _ (hS _ x.property)) _).mp (hu x)
+    · intro T hST hT ⟨u, hu⟩; refine hmax T hST ?_ ?_
+      · exact le_trans hT (extens_monotone hle)
+      · use u; intro x hx; refine (congrFun (hle.form _ ?_) _).mp (hu _ hx)
+        exact extens_subset_nodes _ (hT hx)
+    · ext1 u; refine forall_congr fun x ↦ ?_
+      exact congrFun (hle.form x (hS _ x.property)) _
+
+lemma branches_monotone : @Monotone (Lpofin l) _ _ _ branches := by
+  unfold branches; intro α β hle
+  simp only [Finset.le_eq_subset, Set.Finite.subset_toFinset, Set.Finite.coe_toFinset]
+  exact branches_set_monotone hle
+
+lemma branches_not_mutually_sat {α : Lpofin l} {φ ψ : Form Node}
+    (hφ : φ ∈ α.branches) (hψ : ψ ∈ α.branches) (hneq : φ ≠ ψ) :
+    ∀ v, ¬ (φ v ∧ ψ v) := by
+  intro v ⟨h₁, h₂⟩
+  rcases (Set.Finite.mem_toFinset _).mp hφ with ⟨S, ⟨_, hsub, _, _, hmax⟩, rfl⟩
+  rcases (Set.Finite.mem_toFinset _).mp hψ with ⟨T, ⟨_, hsub', _, _, hmax'⟩, rfl⟩
+  refine hmax (S ∪ T) ⟨Finset.subset_union_left, ?_⟩ ?_ ?_
+  · intro h; apply hneq; refine congrArg _ ?_; ext x; constructor
+    · intro hx; by_contra ht; refine hmax' (insert x T) ?_ ?_ ?_
+      · exact Finset.ssubset_insert ht
+      · intro y hy; rcases Finset.mem_insert.mp hy with rfl | hy
+        · exact hsub hx
+        · exact hsub' hy
+      · use v; intro y hy; rcases Finset.mem_insert.mp hy with rfl | hy
+        · exact h₁ ⟨y, hx⟩
+        · exact h₂ ⟨y, hy⟩
+    · intro hx; exact h (Finset.subset_union_right hx)
+  · intro x hx; rcases Finset.mem_union.mp hx with hx | hx
+    · exact hsub hx
+    · exact hsub' hx
+  · use v; intro x hx; rcases Finset.mem_union.mp hx with hx | hx
+    · exact h₁ ⟨x, hx⟩
+    · exact h₂ ⟨x, hx⟩
+
+end Lpofin
