Pom/Lpo/Operations/Seq/Isomorphism.lean
@@ -1,0 +1,281 @@
+import Pom.Lpo.Operations.Seq
+
+namespace Lpofin
+
+variable {l : Type} [PartialOrder l] [OrderBot l]
+
+lemma branches_permute {α α' : Lpofin l} {e : α.nodes ≃ α'.nodes}
+    (h : α.permute e = α') :
+    ∀ φ ∈ α.branches, φ.permute e ∈ α'.branches := by
+  intro φ hφ
+  obtain ⟨s, ⟨hne, hsub, ⟨v, hsat⟩, hstk, hmax⟩, rfl⟩ := (Set.Finite.mem_toFinset _).mp hφ
+  let t := s.attach.image
+    (fun x : ↑s ↦ (e ⟨x.val, extens_subset_nodes _ (hsub x.property)⟩).val)
+  refine (Set.Finite.mem_toFinset _).mpr ⟨t, ⟨?_, ?_, ?_, ?_, ?_⟩, ?_⟩ <;> subst t
+  · refine Finset.Nonempty.image (Finset.univ_nonempty_iff.mpr ?_) _
+    exact hne.coe_sort
+  · conv => rhs; rw [← h]
+    intro x hx; obtain ⟨⟨y, hy⟩, _, rfl⟩ := Finset.mem_image.mp hx
+    simp only [extens, Finset.mem_filter]; constructor
+    · refine (Set.Finite.mem_toFinset _).mpr ?_; exact Subtype.coe_prop _
+    · intro hc
+      have := hsub hy; simp [extens] at this; have ⟨hy', h'⟩ := this; apply h'
+      have hy' := (Set.Finite.mem_toFinset _).mp hy'; intro v hform
+      have ⟨⟨z, hz, hbot⟩, _, hform'⟩ := hc (Form.image v e) ((Lpo.permute_form_sat_iff hy').mp hform)
+      refine ⟨⟨(e.symm ⟨_, hz⟩).val, Subtype.coe_prop _, ?_⟩, ?_⟩
+      · refine Eq.trans ?_ hbot; exact (if_pos hz).symm
+      · refine (Lpo.permute_form_sat_iff (Subtype.coe_prop _) (e := e)).mpr ?_
+        conv => arg 2; arg 1; exact e.apply_symm_apply _
+        exact ⟨hz, hform'⟩
+  · use Form.image v e; intro ⟨x, hx⟩; obtain ⟨⟨y, hy⟩, _, rfl⟩ := Finset.mem_image.mp hx
+    conv => simp only; arg 1; exact h.symm
+    refine (Lpo.permute_form_sat_iff _).mp (hsat ⟨_, hy⟩)
+  · intro v hv ⟨⟨z, hz, hbot⟩, hform⟩
+    refine hstk (Form.image v e.symm) ?_ ?_
+    · intro ⟨x, hx⟩; refine ((Lpo.permute_form_sat_iff ?_ (e := e)).mpr ?_)
+      · exact extens_subset_nodes _ (hsub hx)
+      · conv => arg 3; arg 2; exact e.symm_symm.symm
+        conv => arg 3; exact Form.image_inv v e.symm
+        refine Lpo.form_inter_nodes_sat_iff.mp ?_
+        conv at hv => arg 1; exact h.symm
+        refine hv ⟨(e ⟨x, _⟩).val, ?_⟩
+        exact Finset.mem_image.mpr ⟨⟨x, hx⟩, Finset.mem_attach _ _, rfl⟩
+    · refine ⟨⟨(e.symm ⟨z, hz⟩).val, Subtype.coe_prop _, ?_⟩, ?_⟩
+      · rw [← h] at hbot; simp only [Lpo.lab, permute, Lpo.permute, dite_eq_right_iff] at hbot
+        exact hbot hz
+      · simp only
+        refine (Lpo.permute_form_sat_iff (Subtype.coe_prop _) (e := e)).mpr ?_
+        conv => arg 3; exact Form.image_inv v e.symm
+        refine Lpo.form_inter_nodes_sat_iff.mp ?_
+        conv => arg 2; simp only [Subtype.coe_eta]; arg 1; exact e.apply_symm_apply _
+        conv at hform => simp only; arg 1; exact h.symm
+        exact hform
+  · intro t ⟨hst, hnts⟩ hex ⟨v, hform⟩
+    refine hmax (t.attach.image fun y ↦ (e.symm ⟨y.val, ?_⟩).val) ?_ ?_ ?_
+    · exact extens_subset_nodes _ (hex y.property)
+    · constructor
+      · intro x hx; refine Finset.mem_image.mpr ⟨⟨e ⟨x, ?_⟩, ?_⟩, Finset.mem_attach _ _, ?_⟩
+        · exact extens_subset_nodes _ (hsub hx)
+        · exact hst (Finset.mem_image.mpr ⟨⟨x, hx⟩, Finset.mem_attach _ _, rfl⟩)
+        · simp only [Subtype.coe_eta, Equiv.symm_apply_apply]
+      · intro hc; apply hnts; intro x hx
+        refine Finset.mem_image.mpr ⟨⟨(e.symm ⟨x, ?_⟩).val, ?_⟩, Finset.mem_attach _ _, ?_⟩
+        · exact extens_subset_nodes _ (hex hx)
+        · exact hc (Finset.mem_image.mpr ⟨⟨x, hx⟩, Finset.mem_attach _ _, rfl⟩)
+        · simp only [Subtype.coe_eta, Equiv.apply_symm_apply]
+    · intro x hx; simp only [extens, Finset.mem_image, Finset.mem_attach, true_and, Finset.mem_filter] at *
+      obtain ⟨y, rfl⟩ := hx; constructor
+      · exact (Set.Finite.mem_toFinset _).mpr (Subtype.coe_prop _)
+      · intro hc; have := hex y.property
+        simp only [extens, nodes_finset, Finset.mem_filter, Set.Finite.mem_toFinset] at this
+        apply this.2; intro v hform
+        rw [← h] at hform; simp only [Lpofin.permute, form, Lpo.permute, Lpo.form] at hform
+        have ⟨hy, hform⟩ := hform
+        have ⟨⟨z, hz, hbot⟩, hform⟩ := hc _ hform
+        refine ⟨⟨(e ⟨_, hz⟩).val, Subtype.coe_prop _, ?_⟩, ?_⟩
+        · conv => arg 1; arg 1; arg 1; exact h.symm
+          simp only [Lpofin.permute, Lpo.permute, Lpo.lab]
+          refine (dif_pos (Subtype.coe_prop _)).trans ?_
+          conv => lhs; arg 2; simp only [Subtype.coe_eta]; arg 1; exact e.symm_apply_apply _
+          exact hbot
+        · simp only [← h]
+          refine Lpo.form_inter_nodes_sat_iff.mpr ?_
+          conv => arg 3; exact (Form.image_inv _ e.symm).symm
+          conv => arg 3; arg 2; exact e.symm_symm
+          exact (Lpo.permute_form_sat_iff _).mp hform
+    · refine ⟨Form.image v e.symm, ?_⟩; intro x hx
+      obtain ⟨y, _, rfl⟩ := Finset.mem_image.mp hx
+      refine (Lpo.permute_form_sat_iff (Subtype.coe_prop _) (e := e)).mpr ?_
+      conv => arg 2; simp only [Subtype.coe_eta]; arg 1; exact e.apply_symm_apply _
+      conv => arg 3; exact Form.image_inv _ _
+      refine Lpo.form_inter_nodes_sat_iff.mp ?_
+      have := hform _ y.property; rw [← h] at this; exact this
+  · conv => lhs; arg 1; rw [← h]
+    simp only [conj]; unfold Form.permute; ext v; constructor
+    · intro hform x
+      have :=
+        hform
+          ⟨(e ⟨x.val, extens_subset_nodes _ (hsub x.property)⟩).val,
+            Finset.mem_image.mpr ⟨x, Finset.mem_attach _ _, rfl⟩⟩
+      simp only [form, Lpo.form, permute, Lpo.permute, Form.permute, Subtype.coe_eta,
+        Subtype.coe_prop, exists_const] at this
+      conv at this => arg 2; arg 1; exact Equiv.symm_apply_apply _ _
+      exact this
+    · intro hform x
+      have ⟨y, _, heq⟩ := Finset.mem_image.mp x.property; rw [← heq]
+      have := hform y
+      simp only [form, Lpo.form, permute, Lpo.permute, Form.permute, Subtype.coe_eta,
+        Subtype.coe_prop, exists_const]
+      conv => arg 2; arg 1; exact Equiv.symm_apply_apply _ _
+      exact this
+
+def branches_equiv {α α' : Lpofin l} {e : α.nodes ≃ α'.nodes}
+    (h : α.permute e = α') :
+    α.branches ≃ α'.branches := {
+  toFun φ := ⟨φ.val.permute e, branches_permute h _ φ.property⟩
+  invFun φ := ⟨φ.val.permute e.symm, by {
+    refine branches_permute ?_ _ φ.property
+    refine Subtype.ext ?_; symm; refine (Lpo.permute_symm ?_)
+    conv => rhs; arg 1; exact h.symm
+    rfl
+  }⟩
+  left_inv := by
+    intro ⟨φ, hφ⟩
+    unfold Form.permute; ext1; ext1 v; simp only [Equiv.symm_symm, Form.image]
+    obtain ⟨s, ⟨_, hsub, _⟩, rfl⟩:= (Set.Finite.mem_toFinset _).mp hφ
+    have h (x : ↑s) := (α.val.property.form _ (extens_subset_nodes _ (hsub x.property))).1
+    refine Form.DependsOn.sAnd h _ _ ?_
+    refine Set.disjoint_left.mpr ?_; intro x hx hx'
+    have ⟨y, hrel⟩ := Set.mem_iUnion.mp hx'
+    rcases Set.mem_symmDiff.mp hx with ⟨⟨z, rfl, w, heq, hw⟩, hv⟩ | ⟨hv, h⟩
+    · apply hv; rw [← Subtype.val_injective heq]; simpa only [Equiv.symm_apply_apply]
+    · have hx := (α.val.property.rel_dom hrel).1
+      refine h ⟨e ⟨x, hx⟩, ?_, ⟨x, hx⟩, rfl, hv⟩
+      simp only [Equiv.symm_apply_apply]
+  right_inv := by
+    intro ⟨φ, hφ⟩
+    unfold Form.permute; ext1; ext1 v; simp only [Form.image, Equiv.symm_symm, Subtype.exists,
+      exists_and_right, Set.mem_setOf_eq, ↓existsAndEq, Subtype.coe_eta, Equiv.apply_symm_apply,
+      Subtype.coe_prop, exists_const, true_and, exists_prop]
+    obtain ⟨s, ⟨_, hsub, _⟩, rfl⟩:= (Set.Finite.mem_toFinset _).mp hφ
+    have h (x : ↑s) := (α'.val.property.form _ (extens_subset_nodes _ (hsub x.property))).1
+    refine Form.DependsOn.sAnd h _ _ ?_
+    refine Set.disjoint_left.mpr ?_; intro x hx hx'
+    have ⟨y, hrel⟩ := Set.mem_iUnion.mp hx'
+    rcases Set.mem_symmDiff.mp hx with ⟨⟨_, h⟩, h'⟩ | ⟨hv, h⟩
+    · exact h' h
+    · refine h ⟨⟨?_, True.intro⟩, hv⟩; exact (α'.val.property.rel_dom hrel).1
+}
+
+lemma seq_isomorphic {α α' β β' : Lpofin l} {f : CopyFn α β} {g : CopyFn α' β'}
+    (hα : α ≈ α') (hβ : β ≈ β') : seq α β f ≈ seq α' β' g := by
+  have ⟨e, he⟩ := hα
+  have eb := branches_equiv (Subtype.ext he)
+  have (φ : ↑α.branches) :
+      ∃ e : ((f φ).nodes ≃ (g (eb φ)).nodes), (f φ).permute e = (g (eb φ)) := by
+    have ⟨ef, hf⟩ := (f.property φ).1
+    have ⟨eg, hg⟩ := (g.property (eb φ)).1
+    have ⟨eβ, h⟩ := hβ
+    refine ⟨ef.trans (eβ.trans eg.symm), ?_⟩
+    unfold Lpofin.permute; refine Subtype.ext ?_; simp only
+    refine Lpo.permute_trans.symm.trans ?_
+    refine Lpo.permute_trans.symm.trans ?_
+    symm; refine Lpo.permute_symm (hg.trans (h.symm.trans ?_))
+    refine Lpo.permute_congr _ _ hf.symm ?_
+    intro x; rfl
+  choose eφ h using this
+  let e' := Equiv.iUnion
+    (fun φ ↦ (f.property φ).2.2)
+    (fun φ ↦ (g.property φ).2.2)
+    eb eφ
+  refine ⟨Equiv.union e e' ?_ ?_ , ?_⟩
+  · refine Set.disjoint_left.mpr ?_; intro x hx hx'
+    have ⟨φ, hx'⟩ := Set.mem_iUnion.mp hx'
+    exact Set.disjoint_left.mp (f.property φ).2.1 hx hx'
+  · refine Set.disjoint_left.mpr ?_; intro x hx hx'
+    have ⟨φ, hx'⟩ := Set.mem_iUnion.mp hx'
+    exact Set.disjoint_left.mp (g.property φ).2.1 hx hx'
+  · ext1
+    · rfl
+    · ext x y
+      by_cases hx : x ∈ (α'.seq β' g).nodes
+      · by_cases hy : y ∈ (α'.seq β' g).nodes
+        · simp only [seq, seq_base, Lpo.permute, Lpo.nodes, Lpo.rel]
+          unfold Rel.permute
+          refine Iff.trans ⟨fun h ↦ h.2.2, fun h ↦ ⟨hx, hy, h⟩⟩ ?_
+          refine or_congr ?_ ?_
+          · unfold Lpofin.rel; rw [← he]
+            simp only [Lpo.permute, Lpo.rel, Rel.permute]
+            constructor
+            · intro hrel; have ⟨hx', hy'⟩ := (α.val.property.rel_dom hrel)
+              have hx := Equiv.mem_union_symm_left hx'
+              have hy := Equiv.mem_union_symm_left hy'
+              refine ⟨hx, hy, ?_⟩
+              rw [Equiv.union_symm_apply_left hx, Equiv.union_symm_apply_left hy] at hrel
+              exact hrel
+            · intro ⟨hx', hy', hrel⟩
+              refine (congrArg₂ α.rel ?_ ?_).mpr hrel
+              · exact Equiv.union_symm_apply_left hx'
+              · exact Equiv.union_symm_apply_left hy'
+          · refine eb.exists_congr ?_; intro φ
+            rw [← h φ]
+            simp only [Lpofin.permute, Lpo.permute, rel, Lpo.rel, nodes, Lpo.nodes, Rel.permute]
+            refine or_congr ?_ ?_
+            · constructor
+              · intro hrel
+                have ⟨hx', hy'⟩ := (f φ).val.property.rel_dom hrel
+                have hx'' := Equiv.mem_union_symm_right (Set.mem_iUnion.mpr ⟨_, hx'⟩)
+                have hy'' := Equiv.mem_union_symm_right (Set.mem_iUnion.mpr ⟨_, hy'⟩)
+                conv at hx' => arg 2; exact Equiv.union_symm_apply_right hx''
+                conv at hy' => arg 2; exact Equiv.union_symm_apply_right hy''
+                unfold e' at hx'
+                have hx := Equiv.mem_iUnion_symm (e := eb) hx'
+                have hy := Equiv.mem_iUnion_symm (e := eb) hy'
+                refine ⟨hx, hy, (congrArg₂ _ ?_ ?_).mp hrel⟩; all_goals {
+                  refine (Equiv.union_symm_apply_right ?_).trans ?_
+                  · assumption
+                  · exact Equiv.iUnion_symm_apply' _
+                }
+              · intro ⟨hx', hy', hrel⟩
+                refine (congrArg₂ _ ?_ ?_).mpr hrel; all_goals {
+                  refine (Equiv.union_symm_apply_right ?_).trans ?_
+                  · refine Set.mem_iUnion.mpr ⟨eb φ, ?_⟩; assumption
+                  · exact Equiv.iUnion_symm_apply' _
+                }
+            · refine and_congr ?_ ?_
+              · sorry
+              · sorry
+        · constructor
+          · intro ⟨_, hy', _⟩; exfalso; exact hy hy'
+          · intro hrel; exfalso; exact hy ((seq _ _ _).val.property.rel_dom hrel).2
+      · constructor
+        · intro ⟨hx', _⟩; exfalso; exact hx hx'
+        · intro hrel; exfalso; exact hx ((seq _ _ _).val.property.rel_dom hrel).1
+    · sorry
+    · sorry
+
+
+
+    --   constructor
+    --   · rintro ⟨hx, hy, hrel | ⟨φ, hrel | ⟨hform, hj⟩⟩⟩
+    --     · left; unfold Lpofin.rel; rw [← he]; simp only [Lpo.permute, Lpo.rel, Rel.permute]
+    --       have ⟨hx', hy'⟩ := (α.val.property.rel_dom hrel)
+    --       have hx := Equiv.mem_union_symm_left hx'
+    --       have hy := Equiv.mem_union_symm_left hy'
+    --       refine ⟨hx, hy, ?_⟩
+    --       rw [Equiv.union_symm_apply_left hx, Equiv.union_symm_apply_left hy] at hrel
+    --       exact hrel
+    --     · right; use eb φ; left
+    --       have ⟨hx', hy'⟩ := (f φ).val.property.rel_dom hrel
+    --       rw [← h φ]; simp only [Lpofin.permute, rel, Lpo.permute, Lpo.rel, Rel.permute]
+    --       sorry
+    --     · sorry
+    --   · intro h; sorry
+    -- · simp only [seq, seq_base, Lpo.permute, Lpo.lab, Lpo.nodes]
+    --   ext x; by_cases hx : x ∈ α'.nodes ∪ ⋃ φ, (g φ).nodes
+    --   · conv => lhs; exact dif_pos hx
+    --     by_cases hx' : ∃ φ, x ∈ (g φ).nodes
+    --     · conv => rhs; exact dif_pos hx'
+    --       have ⟨φ, hx'⟩ := hx'
+    --       refine (dif_pos ?_).trans ?_
+    --       · use eb.symm φ; sorry
+    --       · conv => rhs; arg 1; arg 2; exact (eb.apply_symm_apply _).symm
+    --         conv => rhs; arg 1; exact (h _).symm
+    --         simp only [permute, lab, Lpo.permute, Lpo.lab]
+    --         sorry
+    --   · conv => lhs; exact dif_neg hx
+    --     symm; refine (dif_neg ?_).trans ?_
+    --     · intro ⟨φ, hφ⟩; apply hx; right; exact Set.mem_iUnion.mpr ⟨_, hφ⟩
+    --     · refine α'.val.property.lab_dom _ ?_
+    --       intro hx'; apply hx; left; exact hx'
+    -- · simp only [seq, seq_base, Lpo.permute, Lpo.form, Lpo.nodes]
+    --   ext x v; constructor
+    --   · intro ⟨hx, hform⟩
+    --     rcases hx with hx | hx
+    --     · rw [if_pos hx, Lpofin.form, ← he]
+    --       use hx
+
+    --       --conv => congrFun (if_pos hx) _
+
+
+end Lpofin
